Added some additional structure for UTP theories including top and bottom.

theories/theories/utp_theory.thy
@@ -17,6 +17,8 @@ imports
   "../alpha/utp_alpha_rel"
 begin
 
+subsection {* UTP theories definitions *}
+
 definition is_healthy :: 
   "'a::type \<Rightarrow> ('a \<Rightarrow> 'a) \<Rightarrow> bool" (infix "is" 50) where
 "is_healthy p H \<equiv> H p = p"
@@ -64,18 +66,24 @@ lemma DestTheory_intro [intro]:
   "(\<And> b. DestTheory x = DestTheory y) \<Longrightarrow> x = y"
   by (auto simp add: DestTheory_inject[THEN sym])
 
+lemma DestTheory_elim [elim]:
+  "\<lbrakk> x = y; DestTheory x = DestTheory y \<Longrightarrow> P \<rbrakk> \<Longrightarrow> P"
+  by (auto)
+
 setup_lifting type_definition_WF_THEORY
 
-definition utp_alphabets :: 
+abbreviation utp_alphabets :: 
   "'a WF_THEORY \<Rightarrow> 'a ALPHABET set" ("\<A>") where
-"utp_alphabets t = fst (DestTheory t)"
+"utp_alphabets t \<equiv> fst (DestTheory t)"
 
-definition healthconds :: 
+abbreviation healthconds :: 
   "'a WF_THEORY \<Rightarrow> 'a ALPHA_FUNCTION set" ("\<H>") where
-"healthconds t = snd (DestTheory t)"
+"healthconds t \<equiv> snd (DestTheory t)"
 
-definition THEORY_PRED :: "'a WF_THEORY \<Rightarrow> 'a WF_ALPHA_PREDICATE set" where
+definition THEORY_PRED :: "'a WF_THEORY \<Rightarrow> 'a WF_ALPHA_PREDICATE set" ("\<lbrakk>_\<rbrakk>\<T>") where
 "THEORY_PRED t \<equiv> {p. \<alpha> p \<in> \<A> t \<and>  (\<forall> H \<in> \<H> t. p is H)}"
+
+
 
 instantiation WF_THEORY :: (VALUE) join_semilattice_zero
 begin
@@ -111,5 +119,86 @@ instance
   apply (auto)
 done
 end
+
+abbreviation is_theory_top :: "'a WF_THEORY \<Rightarrow> 'a ALPHABET \<Rightarrow> 'a WF_ALPHA_PREDICATE \<Rightarrow> bool" where
+"is_theory_top T a p \<equiv> (\<alpha> p = a \<and> p \<in> \<lbrakk>T\<rbrakk>\<T> \<and> (\<forall> q \<in> \<lbrakk>T\<rbrakk>\<T>. \<alpha> q = a \<longrightarrow> q \<sqsubseteq> p))"
+
+abbreviation is_theory_bot :: "'a WF_THEORY \<Rightarrow> 'a ALPHABET \<Rightarrow> 'a WF_ALPHA_PREDICATE \<Rightarrow> bool" where
+"is_theory_bot T a p \<equiv> (\<alpha> p = a \<and> p \<in> \<lbrakk>T\<rbrakk>\<T> \<and> (\<forall> q \<in> \<lbrakk>T\<rbrakk>\<T>. \<alpha> q = a \<longrightarrow> p \<sqsubseteq> q))"
+
+definition has_theory_top :: "'a WF_THEORY \<Rightarrow> 'a ALPHABET \<Rightarrow> bool" where
+"has_theory_top T a = (\<exists>! p. is_theory_top T a p)"
+
+definition has_theory_bot :: "'a WF_THEORY \<Rightarrow> 'a ALPHABET \<Rightarrow> bool" where
+"has_theory_bot T a = (\<exists>! p. is_theory_bot T a p)"
+
+definition top_theory :: "'a WF_THEORY \<Rightarrow> 'a ALPHABET \<Rightarrow> 'a WF_ALPHA_PREDICATE" ("\<top>\<^bsub>_[_]\<^esub>") where
+"top_theory T a = (THE p. is_theory_top T a p)"
+
+definition bot_theory :: "'a WF_THEORY \<Rightarrow> 'a ALPHABET \<Rightarrow> 'a WF_ALPHA_PREDICATE" ("\<bottom>\<^bsub>_[_]\<^esub>") where
+"bot_theory T a = (THE p. is_theory_bot T a p)"
+
+subsection {* Theory of relations *}
+
+lift_definition RELH :: "'a ALPHA_FUNCTION"
+is "\<lambda> p. (Abs_fset (\<langle>\<alpha> p\<rangle>\<^sub>f - NON_REL_VAR), \<exists>\<^sub>p NON_REL_VAR. \<pi> p)"
+  by (auto simp add:WF_ALPHA_PREDICATE_def WF_PREDICATE_OVER_def unrest)
+
+lemma RELH_alphabet [alphabet]:
+  "\<alpha> (RELH p) = Abs_fset (\<langle>\<alpha> p\<rangle>\<^sub>f - NON_REL_VAR)"
+  by (simp add:pred_alphabet_def RELH.rep_eq)
+
+lemma EvalA_RELH [evala]:
+  "\<lbrakk>RELH p\<rbrakk>\<pi> = (\<exists>\<^sub>p NON_REL_VAR. \<lbrakk>p\<rbrakk>\<pi>)"
+  by (simp add:EvalA_def RELH.rep_eq)
+
+theorem RELH_idem:
+  "RELH (RELH p) = RELH p"
+  by (utp_alpha_tac, utp_pred_tac)
+
+lemma RELH_REL_ALPHABET:
+  "p is RELH \<longleftrightarrow> \<alpha> p \<in> REL_ALPHABET"
+  apply (auto simp add:RELH.rep_eq is_healthy_def)
+  apply (erule DestPredA_elim)
+  apply (simp add:RELH.rep_eq pred_alphabet_def)
+  apply (case_tac "\<langle>p\<rangle>\<^sub>\<alpha>")
+  apply (force simp add:REL_ALPHABET_def var_defs)[1]
+  apply (utp_alpha_tac, utp_pred_tac)
+  apply (rule)
+  apply (force simp add:REL_ALPHABET_def var_defs)[1]
+  apply (metis (mono_tags) EvalP_UNREST_override UNREST_NON_REL_VAR_WF_RELATION WF_ALPHA_REL_EvalA_WF_RELATION WF_ALPHA_REL_def mem_Collect_eq)
+done
+
+lift_definition REL :: "'a WF_THEORY"
+is "(REL_ALPHABET, {RELH})"
+  by (auto simp add:WF_THEORY_def IDEMPOTENT_OVER_def RELH.rep_eq RELH_idem)
+
+lemma REL_WF_ALPHA_REL:
+  "\<lbrakk>REL\<rbrakk>\<T> = WF_ALPHA_REL"
+  by (simp add:REL.rep_eq THEORY_PRED_def RELH_REL_ALPHABET WF_ALPHA_REL_def)
+
+lemma bot_REL_ALPHABET:
+  "a \<in> REL_ALPHABET \<Longrightarrow> \<bottom>\<^bsub>REL[a]\<^esub> = true\<^bsub>a\<^esub>"
+  apply (auto simp add:bot_theory_def)
+  apply (rule the_equality)
+  apply (simp add:alphabet closure REL_WF_ALPHA_REL)
+  apply (utp_alpha_tac, utp_pred_tac)
+  apply (auto simp add:REL_WF_ALPHA_REL)
+  apply (drule_tac x="true\<^bsub>\<alpha> p\<^esub>" in bspec)
+  apply (simp add:closure)
+  apply (utp_alpha_tac, utp_pred_auto_tac)
+done
+
+lemma top_REL_ALPHABET:
+  "a \<in> REL_ALPHABET \<Longrightarrow> \<top>\<^bsub>REL[a]\<^esub> = false\<^bsub>a\<^esub>"
+  apply (auto simp add:top_theory_def)
+  apply (rule the_equality)
+  apply (simp add:alphabet closure REL_WF_ALPHA_REL)
+  apply (utp_alpha_tac, utp_pred_tac)
+  apply (auto simp add:REL_WF_ALPHA_REL)
+  apply (drule_tac x="false\<^bsub>\<alpha> p\<^esub>" in bspec)
+  apply (simp add:closure)
+  apply (utp_alpha_tac, utp_pred_auto_tac)
+done
 
 end
